disk-betree/ImplMarshalling.i.dfy
@@ -1,0 +1,778 @@
+include "../lib/Marshalling/GenericMarshalling.i.dfy"
+include "ImplState.i.dfy"
+include "ImplModel.i.dfy"
+include "KMTable.i.dfy"
+include "../lib/Option.s.dfy"
+
+include "Marshalling.i.dfy"
+
+module ImplMarshalling {
+  import IM = ImplModel
+  import IMM = Marshalling
+  import opened GenericMarshalling
+  import opened Options
+  import opened NativeTypes
+  import opened Sequences
+  import opened Maps
+  import opened BucketsLib
+  import BC = BetreeGraphBlockCache
+  import ImplState
+  import KMTable
+  import Crypto
+  import Native
+
+  import BT = PivotBetreeSpec`Internal
+
+  import M = ValueMessage`Internal
+  import LBAType
+
+  import Pivots = PivotsLib
+  import MS = MapSpec
+  import Keyspace = MS.Keyspace
+
+  import MM = MutableMap
+
+  type Reference = IMM.Reference
+  type LBA = IMM.LBA
+  type Location = IMM.Location
+  type Sector = IMM.Sector
+  type Message = IMM.Message
+  type Key = IMM.Key
+  type Node = IMM.Node
+
+  /////// Conversion to PivotNode
+
+  method {:fuel ValInGrammar,3} ValToLBAsAndSuccs(a: seq<V>) returns (s : Option<ImplState.MutIndirectionTable>)
+  requires IMM.valToLBAsAndSuccs.requires(a)
+  ensures (
+      && var table := IM.IIndirectionTableOpt(if s.Some? then Some(s.value.Contents) else None);
+      && var inter := IMM.valToLBAsAndSuccs(a);
+      && if table.Some?
+         then (inter.Some? && table.value.locs == inter.value.0 && table.value.graph == inter.value.1)
+         else inter.None?)
+  ensures s.Some? ==> s.value.Inv()
+  ensures s.Some? ==> s.value.Count as nat == |a|
+  ensures s.Some? ==> s.value.Count as nat < 0x10000000000000000 / 8
+  ensures s.Some? ==> fresh(s.value) && fresh(s.value.Repr)
+  {
+    if |a| == 0 {
+      var newHashMap := new MM.ResizingHashMap<(Option<Location>, seq<Reference>)>(1024); // TODO(alattuada) magic numbers
+      s := Some(newHashMap);
+      assume s.value.Count as nat == |a|;
+    } else {
+      var res := ValToLBAsAndSuccs(DropLast(a));
+      match res {
+        case Some(mutMap) => {
+          var tuple := Last(a);
+          var ref := IMM.valToReference(tuple.t[0]);
+          var lba := IMM.valToLBA(tuple.t[1]);
+          var len := tuple.t[2].u;
+          var succs := IMM.valToChildren(tuple.t[3]);
+          match succs {
+            case None => {
+              s := None;
+            }
+            case Some(succs) => {
+              var graphRef := mutMap.Get(ref);
+              var loc := LBAType.Location(lba, len);
+              if graphRef.Some? || lba == 0 || !LBAType.ValidLocation(loc) {
+                s := None;
+              } else {
+                var _ := mutMap.Insert(ref, (Some(loc), succs));
+                s := Some(mutMap);
+                assume s.Some? ==> s.value.Count as nat < 0x10000000000000000 / 8; // TODO(alattuada) removing this results in trigger loop
+                assume s.value.Count as nat == |a|;
+              }
+            }
+          }
+        }
+        case None => {
+          s := None;
+        }
+      }
+    }
+  }
+
+  method GraphClosed(table: ImplState.MutIndirectionTable) returns (result: bool)
+    requires table.Inv()
+    requires BC.GraphClosed.requires(IM.IIndirectionTable(table.Contents).graph)
+    ensures BC.GraphClosed(IM.IIndirectionTable(table.Contents).graph) == result
+  {
+    var m := table.ToMap();
+    var m' := map ref | ref in m :: m[ref].1;
+    result := BC.GraphClosed(m');
+  }
+
+  method ValToIndirectionTable(v: V) returns (s : Option<ImplState.MutIndirectionTable>)
+  requires IMM.valToIndirectionTable.requires(v)
+  ensures IM.IIndirectionTableOpt(if s.Some? then Some(s.value.Contents) else None) == IMM.valToIndirectionTable(v)
+  ensures s.Some? ==> s.value.Inv()
+  {
+    var res := ValToLBAsAndSuccs(v.a);
+    match res {
+      case Some(res) => {
+        var rootRef := res.Get(BT.G.Root());
+        var isGraphClosed := GraphClosed(res);
+        if rootRef.Some? && isGraphClosed {
+          s := Some(res);
+        } else {
+          s := None;
+        }
+      }
+      case None => {
+        s := None;
+      }
+    }
+  }
+
+  lemma valToStrictlySortedKeySeqPrefixNone(v: V, i: int)
+  requires IMM.valToStrictlySortedKeySeq.requires(v)
+  requires 0 <= i <= |v.a|
+  ensures IMM.valToStrictlySortedKeySeq(VArray(v.a[..i])) == None
+      ==> IMM.valToStrictlySortedKeySeq(v) == None
+  decreases |v.a| - i
+  {
+    if (i < |v.a|) {
+      valToStrictlySortedKeySeqPrefixNone(v, i+1);
+      assert DropLast(v.a[..i+1]) == v.a[..i];
+    } else {
+      assert v.a[..i] == v.a;
+    }
+  }
+
+  method ValToStrictlySortedKeySeq(v: V) returns (s : Option<seq<Key>>)
+  requires IMM.valToStrictlySortedKeySeq.requires(v)
+  ensures s == IMM.valToStrictlySortedKeySeq(v)
+  {
+    var ar := new Key[|v.a| as uint64];
+
+    var i: uint64 := 0;
+    while i < |v.a| as uint64
+    invariant 0 <= i as int <= |v.a|
+    invariant IMM.valToStrictlySortedKeySeq(VArray(v.a[..i])) == Some(ar[..i])
+    {
+      assert ValInGrammar(v.a[i], GByteArray);
+      assert ValidVal(v.a[i]);
+
+      valToStrictlySortedKeySeqPrefixNone(v, i as int + 1);
+
+      if |v.a[i].b| as uint64 > Keyspace.MaxLen() {
+        return None;
+      }
+
+      ar[i] := v.a[i].b;
+
+      if (i > 0) {
+        var c := Keyspace.cmp(ar[i-1], ar[i]);
+        if (c >= 0) {
+          assert Last(ar[..i]) == ar[i-1];
+          assert IMM.valToStrictlySortedKeySeq(VArray(v.a[..i+1])) == None;
+
+          return None;
+        }
+      }
+
+      assert DropLast(v.a[..i+1]) == v.a[..i];
+      assert ar[..i+1] == ar[..i] + [ar[i]];
+
+      i := i + 1;
+    }
+
+    assert v.a[..i] == v.a;
+    assert ar[..i] == ar[..];
+    s := Some(ar[..]);
+  }
+
+  method ValToPivots(v: V) returns (s : Option<seq<Key>>)
+  requires IMM.valToPivots.requires(v)
+  ensures s == IMM.valToPivots(v)
+  {
+    s := ValToStrictlySortedKeySeq(v);
+    if (s.Some? && |s.value| as uint64 > 0 && |s.value[0]| as uint64 == 0) {
+      s := None;
+    }
+  }
+
+  method ValToBucket(v: V, pivotTable: seq<Key>, i: int) returns (s : Option<KMTable.KMTable>)
+  requires IMM.valToBucket.requires(v, pivotTable, i)
+  ensures s.Some? ==> KMTable.WF(s.value)
+  ensures s.Some? ==> KMTable.Bounded(s.value)
+  ensures s.Some? ==> WFBucketAt(KMTable.I(s.value), pivotTable, i)
+  ensures IMM.IKMTableOpt(s) == IMM.valToBucket(v, pivotTable, i)
+  {
+    assert ValidVal(v.t[0]);
+    if (|v.t[0].a| as uint64 >= KMTable.MaxNumKeys()) {
+      return None;
+    }
+
+    var keys := ValToStrictlySortedKeySeq(v.t[0]);
+
+    if keys.None? {
+      return None;
+    }
+
+    var values := IMM.valToMessageSeq(v.t[1]);
+
+    if values.None? {
+      return None;
+    }
+
+    var kmt := KMTable.KMTable(keys.value, values.value);
+
+    var wf := KMTable.IsWF(kmt);
+    if !wf {
+      return None;
+    }
+
+    // Check that it fits in the desired bucket
+    if |kmt.keys| > 0 {
+      if i > 0 {
+        var c := Keyspace.cmp(pivotTable[i-1], kmt.keys[0]);
+        if (c > 0) {
+          KMTable.Imaps(kmt, 0);
+          return None;
+        }
+      }
+
+      if i < |pivotTable| {
+        var c := Keyspace.cmp(pivotTable[i], kmt.keys[|kmt.keys| - 1]);
+        if (c <= 0) {
+          KMTable.Imaps(kmt, |kmt.keys| - 1);
+          return None;
+        }
+      }
+    }
+
+    forall key | key in KMTable.I(kmt)
+    ensures Pivots.Route(pivotTable, key) == i
+    ensures KMTable.I(kmt)[key] != M.IdentityMessage()
+    {
+      var j := KMTable.IndexOfKey(kmt, key);
+      KMTable.Imaps(kmt, j);
+      if |kmt.keys| > 0 {
+        Keyspace.IsStrictlySortedImpliesLte(kmt.keys, 0, j);
+        Keyspace.IsStrictlySortedImpliesLte(kmt.keys, j, |kmt.keys| - 1);
+      }
+      Pivots.RouteIs(pivotTable, key, i);
+    }
+
+    assert WFBucketAt(KMTable.I(kmt), pivotTable, i);
+    s := Some(kmt);
+  }
+
+  lemma LemmaValToBucketNone(a: seq<V>, pivotTable: seq<Key>, i: int)
+  requires Pivots.WFPivots(pivotTable)
+  requires forall i | 0 <= i < |a| :: ValidVal(a[i])
+  requires forall i | 0 <= i < |a| :: ValInGrammar(a[i], IMM.BucketGrammar())
+  requires |a| <= |pivotTable| + 1
+  requires 0 <= i < |a|
+  requires IMM.valToBucket(a[i], pivotTable, i) == None
+  ensures IMM.valToBuckets(a, pivotTable) == None
+  {
+    if (|a| == i + 1) {
+    } else {
+      LemmaValToBucketNone(DropLast(a), pivotTable, i);
+    }
+  }
+
+  method ValToBuckets(a: seq<V>, pivotTable: seq<Key>) returns (s : Option<seq<KMTable.KMTable>>)
+  requires IMM.valToBuckets.requires(a, pivotTable)
+  ensures s.Some? ==> IM.WFBuckets(s.value)
+  ensures IMM.ISeqKMTableOpt(s) == IMM.valToBuckets(a, pivotTable)
+  {
+    var ar := new KMTable.KMTable[|a|];
+
+    var i := 0;
+    while i < |a|
+    invariant 0 <= i <= |a|
+    invariant forall k: nat | k < i :: KMTable.WF(ar[k])
+    invariant forall k: nat | k < i :: KMTable.Bounded(ar[k])
+    invariant forall k: nat | k < i :: WFBucketAt(KMTable.I(ar[k]), pivotTable, k)
+    invariant IMM.valToBuckets(a[..i], pivotTable).Some?
+    invariant Apply(KMTable.I, ar[..i]) == IMM.valToBuckets(a[..i], pivotTable).value
+    {
+      var b := ValToBucket(a[i], pivotTable, i);
+      if (b.None?) {
+        s := None;
+
+        LemmaValToBucketNone(a, pivotTable, i);
+        return;
+      }
+
+      ar[i] := b.value;
+
+      assert DropLast(a[..i+1]) == a[..i];
+      assert ar[..i+1] == ar[..i] + [b.value];
+
+      i := i + 1;
+    }
+
+    assert a[..|a|] == a;
+    assert ar[..|a|] == ar[..];
+
+    assert IMM.valToBuckets(a[..], pivotTable).Some?;
+    assert Apply(KMTable.I, ar[..]) == IMM.valToBuckets(a, pivotTable).value;
+
+    s := Some(ar[..]);
+  }
+
+  method ValToNode(v: V) returns (s : Option<ImplState.Node>)
+  requires IMM.valToNode.requires(v)
+  ensures s.Some? ==> IM.WFNode(s.value)
+  ensures IMM.INodeOpt(s) == IMM.valToNode(v)
+  {
+    assert ValidVal(v.t[0]);
+    var pivotsOpt := ValToPivots(v.t[0]);
+    if (pivotsOpt.None?) {
+      return None;
+    }
+    var pivots := pivotsOpt.value;
+
+    var childrenOpt := IMM.valToChildren(v.t[1]);
+    if (childrenOpt.None?) {
+      return None;
+    }
+    var children := childrenOpt.value;
+
+    if (!((|children| == 0 || |children| == |pivots| + 1) && |v.t[2].a| == |pivots| + 1)) {
+      return None;
+    }
+
+    assert ValidVal(v.t[2]);
+    var bucketsOpt := ValToBuckets(v.t[2].a, pivots);
+    if (bucketsOpt.None?) {
+      return None;
+    }
+    var buckets := bucketsOpt.value;
+
+    var node := IM.Node(pivots, if |children| == 0 then None else childrenOpt, buckets);
+
+    assert IMM.valToNode(v).Some?;
+    assert IM.WFBuckets(node.buckets);
+    assert IM.INode(node) == IMM.valToNode(v).value;
+    return Some(node);
+  }
+
+  method ValToSector(v: V) returns (s : Option<ImplState.Sector>)
+  requires IMM.valToSector.requires(v)
+  ensures s.Some? ==> ImplState.WFSector(s.value)
+  ensures s.Some? ==> IM.WFSector(ImplState.ISector(s.value))
+  ensures IMM.ISectorOpt(s) == IMM.valToSector(v)
+  {
+    if v.c == 0 {
+      var mutMap := ValToIndirectionTable(v.val);
+      match mutMap {
+        case Some(s) => return Some(ImplState.SectorIndirectionTable(s));
+        case None => return None;
+      }
+    } else {
+      var node := ValToNode(v.val);
+      match node {
+        case Some(s) => return Some(ImplState.SectorBlock(s));
+        case None => return None;
+      }
+    }
+  }
+
+  /////// Conversion from PivotNode to a val
+
+  method childrenToVal(children: seq<Reference>) returns (v : V)
+  requires |children| < 0x1_0000_0000_0000_0000
+  ensures ValidVal(v)
+  ensures SizeOfV(v) <= 8 + |children| * 8
+  ensures ValInGrammar(v, GUint64Array)
+  ensures IMM.valToChildren(v) == Some(children)
+  ensures |v.ua| == |children|
+  {
+    return VUint64Array(children);
+  }
+
+  method {:fuel ValInGrammar,2} lbasSuccsToVal(locs: map<Reference, Location>, graph: map<Reference, seq<Reference>>) returns (v: Option<V>)
+  requires locs.Keys == graph.Keys
+  requires forall loc | loc in locs.Values :: BC.ValidLocationForNode(loc)
+  requires |locs| < 0x1_0000_0000_0000_0000 / 8
+  ensures v.Some? ==> ValidVal(v.value)
+  ensures v.Some? ==> ValInGrammar(v.value, IMM.IndirectionTableGrammar());
+  ensures v.Some? ==> |v.value.a| == |locs|
+  ensures v.Some? ==> IMM.valToLBAsAndSuccs(v.value.a) == Some((locs, graph));
+  {
+    if (|locs| == 0) {
+      assert locs == map[];
+      assert graph == map[];
+      return Some(VArray([]));
+    } else {
+      var ref :| ref in locs.Keys;
+      var vpref := lbasSuccsToVal(MapRemove(locs, {ref}), MapRemove(graph, {ref}));
+      match vpref {
+        case None => return None;
+        case Some(vpref) => {
+          var loc := locs[ref];
+          if (|graph[ref]| >= 0x1_0000_0000_0000_0000) {
+            return None;
+          }
+          var succs := childrenToVal(graph[ref]);
+          var tuple := VTuple([IMM.refToVal(ref), IMM.lbaToVal(loc.addr), VUint64(loc.len), succs]);
+
+          assert MapRemove(locs, {ref})[ref := loc] == locs;
+          assert MapRemove(graph, {ref})[ref := graph[ref]] == graph;
+
+          //assert ref == valToReference(tuple.t[0]);
+          //assert lba == valToReference(tuple.t[1]);
+          //assert !(ref in MapRemove(graph, {ref}));
+          assert BC.ValidLocationForNode(loc);
+          //assert !(lba == 0);
+          //assert valToLBAsAndSuccs(vpref.a + [tuple]) == Some((lbas, graph));
+          assert ValidVal(tuple);
+
+          return Some(VArray(vpref.a + [tuple]));
+        }
+      }
+    }
+  }
+
+  method {:fuel ValidVal,2} uint64ArrayToVal(a: seq<uint64>) returns (v: V)
+  requires |a| < 0x1_0000_0000_0000_0000
+  ensures ValidVal(v)
+  ensures ValInGrammar(v, GUint64Array)
+  ensures SizeOfV(v) == 8 + 8 * |a|
+  ensures |v.ua| == |a|
+  ensures IMM.valToUint64Seq(v) == a
+  {
+    return VUint64Array(a);
+  }
+
+  method strictlySortedKeySeqToVal(keys: seq<Key>) returns (v : V)
+  requires Keyspace.IsStrictlySorted(keys)
+  requires |keys| < 0x1_0000_0000_0000_0000
+  ensures ValidVal(v)
+  ensures SizeOfV(v) <= 8 + |keys| * (8 + IMM.CapKeySize() as int)
+  ensures ValInGrammar(v, GArray(GByteArray))
+  ensures |v.a| == |keys|
+  ensures IMM.valToStrictlySortedKeySeq(v) == Some(keys)
+  {
+    var ar := new V[|keys| as uint64];
+    var i: uint64 := 0;
+    while i < |keys| as uint64
+    invariant i as int <= |keys|
+    invariant ValidVal(VArray(ar[..i]))
+    invariant SizeOfV(VArray(ar[..i])) as int <= 8 + i as int * (8 + IMM.CapKeySize() as int)
+    invariant ValInGrammar(VArray(ar[..i]), GArray(GByteArray))
+    invariant IMM.valToStrictlySortedKeySeq(VArray(ar[..i])) == Some(keys[..i])
+    {
+      ar[i] := VByteArray(keys[i]);
+
+      lemma_SeqSum_prefix(ar[..i], VByteArray(keys[i]));
+      assert keys[..i+1][..i] == keys[..i];
+      assert ar[..i+1][..i] == ar[..i];
+      assert ar[..i+1] == ar[..i] + [ar[i]];
+      assert keys[..i] + [keys[i]] == keys[..i+1];
+
+      if i > 0 {
+        Keyspace.IsStrictlySortedImpliesLt(keys, i as int - 1, i as int);
+      }
+
+      assert i > 0 ==> keys[i-1] == Last(DropLast(keys[..i as int + 1]));
+      assert keys[i] == Last(keys[..i as int + 1]);
+
+      i := i + 1;
+    }
+    v := VArray(ar[..]);
+
+    assert ar[..i] == ar[..];
+    assert keys[..i] == keys;
+  }
+
+  lemma KeyInPivotsIsNonempty(pivots: seq<Key>)
+  requires Pivots.WFPivots(pivots)
+  requires |pivots| > 0
+  ensures |pivots[0]| != 0;
+  {
+    var e := Keyspace.SmallerElement(pivots[0]);
+    Keyspace.reveal_seq_lte();
+  }
+
+  method pivotsToVal(pivots: seq<Key>) returns (v : V)
+  requires Pivots.WFPivots(pivots)
+  requires |pivots| <= IMM.CapNumBuckets() as int - 1
+  ensures ValidVal(v)
+  ensures SizeOfV(v) <= 8 + |pivots| * (8 + IMM.CapKeySize() as int)
+  ensures ValInGrammar(v, GArray(GByteArray))
+  ensures |v.a| == |pivots|
+  ensures IMM.valToPivots(v) == Some(pivots)
+  {
+    v := strictlySortedKeySeqToVal(pivots);
+
+    if |pivots| > 0 {
+      KeyInPivotsIsNonempty(pivots);
+    }
+  }
+
+  method messageSeqToVal(s: seq<Message>) returns (v : V)
+  requires |s| <= IMM.CapBucketNumEntries() as int
+  requires forall i | 0 <= i < |s| :: s[i] != M.IdentityMessage()
+  requires forall i | 0 <= i < |s| :: IMM.MessageSize(s[i]) <= IMM.CapValueSize() as int
+  ensures ValidVal(v)
+  ensures ValInGrammar(v, GArray(GByteArray))
+  ensures SizeOfV(v) <= 8 + (8 + IMM.CapValueSize()) as int * IMM.CapBucketNumEntries() as int
+  ensures |v.a| == |s|
+  ensures IMM.valToMessageSeq(v) == Some(s)
+  {
+    var ar := new V[|s| as uint64];
+    var i: uint64 := 0;
+    while i < |s| as uint64
+    invariant 0 <= i <= |s| as uint64
+    invariant ValidVal(VArray(ar[..i]))
+    invariant ValInGrammar(VArray(ar[..i]), GArray(GByteArray))
+    invariant IMM.valToMessageSeq(VArray(ar[..i])) == Some(s[..i])
+    invariant SizeOfV(VArray(ar[..i])) <= 8 + (8 + IMM.CapValueSize()) as int * i as int
+    {
+      ar[i] := VByteArray(s[i].value);
+
+      lemma_SeqSum_prefix(ar[..i], VByteArray(s[i].value));
+      assert s[..i+1][..i] == s[..i];
+      assert ar[..i+1][..i] == ar[..i];
+      assert ar[..i+1] == ar[..i] + [ar[i]];
+      assert s[..i] + [s[i]] == s[..i+1];
+
+      i := i + 1;
+    }
+    v := VArray(ar[..]);
+
+    assert ar[..i] == ar[..];
+    assert s[..i] == s;
+  }
+
+  // We pass in pivotTable and i so we can state the pre- and post-conditions.
+  method {:fuel SizeOfV,3}
+  bucketToVal(bucket: KMTable.KMTable, ghost pivotTable: Pivots.PivotTable, ghost i: int) returns (v: V)
+  requires Pivots.WFPivots(pivotTable)
+  requires KMTable.WF(bucket)
+  requires WFBucketAt(KMTable.I(bucket), pivotTable, i)
+  requires IMM.CappedBucket(bucket)
+  requires 0 <= i <= |pivotTable|
+  ensures ValInGrammar(v, IMM.BucketGrammar())
+  ensures SizeOfV(v) <= (8 + (8+IMM.CapKeySize() as int) * IMM.CapBucketNumEntries() as int) + (8 + (8+IMM.CapValueSize() as int) * IMM.CapBucketNumEntries() as int)
+  ensures ValidVal(v)
+  ensures IMM.valToBucket(v, pivotTable, i) == IMM.IKMTableOpt(Some(bucket))
+  {
+    var keys := strictlySortedKeySeqToVal(bucket.keys);
+    var values := messageSeqToVal(bucket.values);
+    v := VTuple([keys, values]);
+
+    // FIXME dafny goes nuts with trigger loops here some unknown reason
+    // without these obvious asserts.
+    assert ValInGrammar(v.t[0], IMM.BucketGrammar().t[0]);
+    assert ValInGrammar(v.t[1], IMM.BucketGrammar().t[1]);
+    assert ValInGrammar(v, IMM.BucketGrammar());
+  }
+
+  method bucketsToVal(buckets: seq<KMTable.KMTable>, ghost pivotTable: Pivots.PivotTable) returns (v: V)
+  requires Pivots.WFPivots(pivotTable)
+  requires forall i | 0 <= i < |buckets| :: KMTable.WF(buckets[i])
+  requires forall i | 0 <= i < |buckets| :: WFBucketAt(KMTable.I(buckets[i]), pivotTable, i)
+  requires IMM.CappedBuckets(buckets)
+  requires |buckets| <= IMM.CapNumBuckets() as int
+  requires |buckets| <= |pivotTable| + 1
+  ensures ValidVal(v)
+  ensures SizeOfV(v) <= 8 + |buckets| * ((8 + (8+IMM.CapKeySize()) as int * IMM.CapBucketNumEntries() as int) + (8 + (8+IMM.CapValueSize()) as int * IMM.CapBucketNumEntries() as int))
+  ensures ValInGrammar(v, GArray(IMM.BucketGrammar()))
+  ensures |v.a| == |buckets|
+  ensures IMM.valToBuckets(v.a, pivotTable) == IMM.ISeqKMTableOpt(Some(buckets))
+  {
+    if |buckets| == 0 {
+      return VArray([]);
+    } else {
+      var pref := bucketsToVal(DropLast(buckets), pivotTable);
+      var bucket := Last(buckets);
+      var bucketVal := bucketToVal(bucket, pivotTable, |buckets| - 1);
+      assert buckets == DropLast(buckets) + [Last(buckets)]; // observe
+      lemma_SeqSum_prefix(pref.a, bucketVal);
+      assert IMM.valToBuckets(VArray(pref.a + [bucketVal]).a, pivotTable).Some?; // observe
+      assert IMM.valToBuckets(VArray(pref.a + [bucketVal]).a, pivotTable).value == Apply(KMTable.I, buckets); // observe
+      assert IMM.valToBuckets(VArray(pref.a + [bucketVal]).a, pivotTable) == IMM.ISeqKMTableOpt(Some(buckets)); // observe (reduces verification time)
+      return VArray(pref.a + [bucketVal]);
+    }
+  }
+
+  method {:fuel SizeOfV,4} nodeToVal(node: ImplState.Node) returns (v : V)
+  requires IM.WFNode(node)
+  requires BT.WFNode(IM.INode(node))
+  requires IMM.CappedNode(node)
+  ensures ValidVal(v)
+  ensures SizeOfV(v) <= 
+      8 + IMM.CapNumBuckets() as int * ((8 + (8+IMM.CapKeySize()) as int * IMM.CapBucketNumEntries() as int) + (8 + (8+IMM.CapValueSize()) as int * IMM.CapBucketNumEntries() as int)) +
+      8 + (IMM.CapNumBuckets() as int - 1) * (8 + IMM.CapKeySize() as int) +
+      8 + IMM.CapNumBuckets() as int * 8
+  ensures ValInGrammar(v, IMM.PivotNodeGrammar())
+  ensures IMM.valToNode(v) == IMM.INodeOpt(Some(node))
+  {
+    var buckets := bucketsToVal(node.buckets, node.pivotTable);
+
+    var pivots := pivotsToVal(node.pivotTable);
+
+    var children;
+    if node.children.Some? {
+      children := childrenToVal(node.children.value);
+    } else {
+      children := VUint64Array([]);
+    }
+      
+    v := VTuple([pivots, children, buckets]);
+
+    assert SizeOfV(v) == SizeOfV(pivots) + SizeOfV(children) + SizeOfV(buckets);
+    assert IMM.valToNode(v).Some?;
+    assert IMM.valToNode(v).value == IM.INode(node);
+  }
+
+  method sectorToVal(sector: ImplState.Sector) returns (v : Option<V>)
+  requires ImplState.WFSector(sector)
+  requires IM.WFSector(ImplState.ISector(sector))
+  requires sector.SectorBlock? ==> BT.WFNode(IM.INode(sector.block))
+  requires sector.SectorBlock? ==> IMM.CappedNode(sector.block);
+  requires sector.SectorIndirectionTable? ==>
+      BC.WFCompleteIndirectionTable(IM.IIndirectionTable(sector.indirectionTable.Contents))
+  ensures v.Some? ==> ValidVal(v.value)
+  ensures v.Some? ==> ValInGrammar(v.value, IMM.SectorGrammar());
+  ensures v.Some? ==> IMM.valToSector(v.value) == IMM.ISectorOpt(Some(sector))
+  ensures sector.SectorBlock? ==> v.Some?
+  ensures sector.SectorBlock? ==> SizeOfV(v.value) <= IMM.BlockSize() as int - 32
+  {
+    match sector {
+      case SectorIndirectionTable(mutMap) => {
+        var table := mutMap.ToMap();
+        // TODO(alattuada) extract to method
+        var lbas := map k | k in table && table[k].0.Some? :: table[k].0.value;
+        var graph := map k | k in table :: table[k].1;
+        assert table == mutMap.Contents;
+        ghost var indirectionTable := IM.IIndirectionTable(mutMap.Contents);
+        assert lbas == indirectionTable.locs;
+        assert graph == indirectionTable.graph;
+        assert lbas.Keys == graph.Keys;
+        if |lbas| < 0x1_0000_0000_0000_0000 / 8 {
+          var w := lbasSuccsToVal(lbas, graph);
+          match w {
+            case Some(v) => return Some(VCase(0, v));
+            case None => return None;
+          }
+        } else {
+          return None;
+        }
+      }
+      case SectorBlock(node) => {
+        var v := nodeToVal(node);
+        return Some(VCase(1, v));
+      }
+    }
+  }
+
+  /////// Marshalling and de-marshalling
+
+  method ParseSector(data: seq<byte>, start: uint64) returns (s : Option<Sector>)
+  requires start as int <= |data| < 0x1_0000_0000_0000_0000;
+  ensures s.Some? ==> ImplState.WFSector(s.value)
+  ensures s.Some? ==> IM.WFSector(ImplState.ISector(s.value))
+  ensures IMM.ISectorOpt(s) == IMM.parseSector(data[start..])
+  ensures s.Some? && s.value.SectorBlock? ==> BT.WFNode(IM.INode(s.value.block))
+  {
+    IMM.reveal_parseSector();
+    var success, v, rest_index := ParseVal(data, start, IMM.SectorGrammar());
+    if success {
+      var s := ValToSector(v);
+      return s;
+    } else {
+      return None;
+    }
+  }
+
+  method MarshallIntoFixedSize(val:V, grammar:G, start: uint64, n: uint64) returns (data:array<byte>)
+    requires ValidGrammar(grammar);
+    requires ValInGrammar(val, grammar);
+    requires ValidVal(val);
+    requires start <= n
+    requires 0 <= SizeOfV(val) <= n as int - start as int
+    ensures fresh(data);
+    ensures |data[..]| == n as int
+    ensures parse_Val(data[start..], grammar).0.Some? && parse_Val(data[start..], grammar).0.value == val;
+  {
+    data := new byte[n];
+    var computed_size := GenericMarshalling.MarshallVal(val, grammar, data, start);
+    //print "computed_size "; print computed_size; print "\n";
+    GenericMarshalling.lemma_parse_Val_view_specific(data[..], val, grammar, start as int, (n as int));
+    assert data[start..] == data[start..n];
+  }
+
+  /////// Marshalling and de-marshalling with checksums
+
+  method ParseCheckedSector(data: seq<byte>) returns (s : Option<Sector>)
+  requires |data| < 0x1_0000_0000_0000_0000;
+  ensures s.Some? ==> ImplState.WFSector(s.value)
+  ensures s.Some? ==> IM.WFSector(ImplState.ISector(s.value))
+  ensures IMM.ISectorOpt(s) == IMM.parseCheckedSector(data[..])
+  ensures s.Some? && s.value.SectorBlock? ==> BT.WFNode(IM.INode(s.value.block))
+  {
+    s := None;
+
+    if |data| as uint64 >= 32 {
+      var hash := Crypto.Crc32(data[32..]);
+      if hash == data[..32] {
+        s := ParseSector(data, 32);
+      }
+    }
+
+    IMM.reveal_parseCheckedSector();
+  }
+
+  method MarshallCheckedSector(sector: Sector) returns (data : array?<byte>)
+  requires ImplState.WFSector(sector)
+  requires IM.WFSector(ImplState.ISector(sector))
+  requires sector.SectorBlock? ==> BT.WFNode(IM.INode(sector.block))
+  requires sector.SectorBlock? ==> IMM.CappedNode(sector.block);
+  ensures data != null ==> IMM.parseCheckedSector(data[..]) == IMM.ISectorOpt(Some(sector))
+  ensures data != null ==> data.Length <= IMM.BlockSize() as int
+  ensures data != null ==> 32 <= data.Length
+  ensures data != null && sector.SectorIndirectionTable? ==> data.Length == IMM.BlockSize() as int
+  ensures sector.SectorBlock? ==> data != null;
+  {
+    var v := sectorToVal(sector);
+    match v {
+      case None => return null;
+      case Some(v) => {
+        if (SizeOfV(v) <= IMM.BlockSize() as int - 32) {
+          //Native.BenchmarkingUtil.start();
+          var size: uint64;
+          if (sector.SectorIndirectionTable?) {
+            size := IMM.BlockSize();
+          } else {
+            var computedSize := GenericMarshalling.ComputeSizeOf(v);
+            size := 32 + computedSize;
+          }
+
+          var data := MarshallIntoFixedSize(v, IMM.SectorGrammar(), 32, size);
+          //Native.BenchmarkingUtil.end();
+
+          IMM.reveal_parseSector();
+          IMM.reveal_parseCheckedSector();
+
+          var hash := Crypto.Crc32Array(data, 32, data.Length as uint64 - 32);
+          assert data[32..] == data[32..data.Length];
+          assert hash == Crypto.Crc32(data[32..]);
+          ghost var data_suffix := data[32..];
+          Native.Arrays.CopySeqIntoArray(hash, 0, data, 0, 32);
+          assert data_suffix == data[32..];
+
+          /*ghost var data_seq := data[..];
+          assert |data_seq| >= 32;
+          assert Crypto.Crc32(data_seq[32..])
+              == Crypto.Crc32(data[32..])
+              == hash
+              == data[..32]
+              == data_seq[..32];*/
+
+          return data;
+        } else {
+          return null;
+        }
+      }
+    }
+  }
+}
